SPLean/Experiments/List.lean
@@ -1,0 +1,153 @@
+import Mathlib.Data.Int.Interval
+import Mathlib.Tactic
+
+import SPLean.Theories.WP1
+import SPLean.Theories.Lang
+import SPLean.Theories.ArraysFun
+import SPLean.Theories.Records
+
+
+section find_index
+
+open Theories prim val trm
+
+
+def fst: field := 0
+def snd : field := 1
+
+
+
+/- First we put simple triple lemmas into our hint data base
+   Those lemmas tell how to symbolically advance basic language instructions -/
+
+#hint_xapp triple_get
+#hint_xapp triple_lt
+#hint_xapp triple_sub
+#hint_xapp triple_neq
+#hint_xapp triple_arrayFun_length
+#hint_xapp triple_harrayFun_get
+
+
+namespace Lang
+
+
+def MList (L: List val) (p:loc) : hProp :=
+  match L with
+  | List.nil => ⌜p = null⌝
+  | List.cons x L' => ∃ʰ (q:loc), (p ~~~> `{ head := x; tail := q}) ∗ (MList L' q)
+
+lemma MList_nil : ∀ p,
+  (MList List.nil p) = ⌜p = null⌝ :=
+by aesop
+
+lemma MList_cons : ∀ p x L',
+  MList (x::L') p = ∃ʰ (q:loc), (p ~~~> `{ head := x; tail := q}) ∗ (MList L' q) :=
+by aesop
+
+
+lemma MList_if : ∀ (p:loc) (L:List val),
+      (MList L p)
+  ==> (if p = null
+        then ⌜L = []⌝
+        else ∃ʰ x, ∃ʰ (q:loc), ∃ʰ L',
+        ⌜L = x::L'⌝ ∗ (p ~~~> `{ head := x; tail := q}) ∗ (MList L' q)) := by sorry
+
+
+lang_def mnil:= fun u => null
+
+lemma triple_mnil :
+  triple [lang| mnil () ]
+  (⌜True⌝)
+  (funloc p ↦ (MList (List.nil) p) ) :=
+by
+  xval
+  xsimp
+  { aesop }
+  { intro; dsimp[MList_nil null]; xsimp }
+
+
+
+axiom well_founded_ind (A : Type) (R : A -> A -> Prop):
+  ∀ P:A -> Prop,
+    (forall x:A, (forall y:A, R y x -> P y) -> P x) -> ∀ a:A, P a
+
+inductive list_sub : (List val) -> (List val) -> Prop where
+| exact (x : val) (L' : List val) : list_sub L' (x::L')
+
+
+
+
+#check tail
+
+lang_def append := fix f p1 p2 =>
+       let q1 := ⟨val_get_field tail⟩ p1 in
+       let b := (q1 = null) in
+       if b
+         then ⟨val_set_field tail⟩ p1 p2
+         else f q1 p2
+
+
+
+
+lemma triple_append (p1 p2 : loc) (L1 L2 : List val): ¬(p1 = null) →
+(triple  [lang| append p1 p2 ] ((MList L1 p1) ∗ (MList L2 p2))
+(fun _ =>  (MList (L1++L2) p1))) :=
+by
+  intro N
+  revert p1
+  induction L1 with
+  | nil =>
+    intro p1 contra
+    xwp
+    xchange (MList_if p1)
+    scase_if
+    {intro H; simp[contra] at H }
+    { intro H; xpull; intro _ _ _ contra; simp at contra }
+  | cons x' L' ih =>
+    intro p1 H
+    xwp
+    xchange (MList_if p1)
+    scase_if
+    { intro H1; simp[H] at H1}
+    { intro H1
+      xpull
+      intro x q1 L1' HH
+      simp at HH
+      simp[HH]
+      xapp triple_get_field_hrecord
+      xwp
+      xchange (MList_if q1)
+      xapp triple_eq
+      simp[is_true]
+      scase_if
+      {
+        intro Hq1
+        xif
+        {
+          intro is_true
+          xapp triple_set_field_hrecord
+          simp[MList_cons]
+          xsimp
+        }
+        {
+          intro contra
+          simp at contra
+        }
+      }
+      {
+        intro h
+        xif
+        { intro contra; simp at contra }
+        {
+           intro _
+           xpull
+           intro x_1 q L'_1 hs
+           simp[XSimp]
+           xsimp
+           simp[MList]
+           xapp (ih)
+           simp[hs, MList]
+           xsimp
+        }
+      }
+    }
