SPLean/Theories/Records.lean
@@ -1,0 +1,479 @@
+import SPLean.Theories.XSimp
+import SPLean.Theories.XChange
+import SPLean.Common.Util
+import SPLean.Theories.SepLog
+import SPLean.Theories.WP1
+import SPLean.Theories.Lang
+import SPLean.Theories.Arrays
+
+open Classical
+
+
+open trm val Theories
+
+
+abbrev field : Type := ℕ
+
+
+
+
+
+def hfield (p : loc) (k : field) (v : val) : hProp  :=
+  (p + 1 + k) ~~> v
+
+notation:100 p:100 ". " k:100 " ~~> " v:0 => hfield p k v
+
+abbrev hrecord_field: Type := field × val
+abbrev hrecord_fields : Type := List hrecord_field
+
+
+notation "`{" k1 " := " v1 "}" => [(k1, (v1 : val))]
+notation "`{" k1 " := " v1 "; " k2 " := " v2 "}" => [(k1, (v1 : val)), (k2, (v2 : val))]
+notation "`{" k1 " := " v1 "; " k2 " := " v2 "; " k3 " := " v3 "}" => [(k1, (v1 : val)), (k2, (v2 : val)), (k3, (v3 : val))]
+
+def hfields (kvs : hrecord_fields) (p:loc): hProp :=
+  match kvs with
+  | [] => ⌜True⌝
+  | (ki, vi) :: kvs' => (p. ki ~~> vi) ∗ (hfields kvs' p)
+-- axiom hrecord : hrecord_fields → loc → hProp
+
+
+--notation p " ~~~> " kvs => hrecord kvs p
+
+--axiom hrecord_not_null : ∀ (p : loc) (kvs : hrecord_fields), hrecord kvs p ==> hrecord kvs p ∗  ⌜p ≠ null⌝
+
+-- Read Operation on Record fields
+--axiom val_get_field : field → val
+
+
+
+
+def maps_all_fields (n:ℕ) (kvs:hrecord_fields) : Prop :=
+  List.map Prod.fst kvs =  List.range' 0 n
+
+def hrecord (kvs:hrecord_fields) (p:loc) : hProp :=
+  ∃ʰ (n:ℕ), hheader n p ∗ hfields kvs p ∗ ⌜maps_all_fields n kvs⌝
+
+notation p " ~~~> " kvs => hrecord kvs p
+
+lemma hrecord_elim_aux (kvs:hrecord_fields)
+ :
+  ∀ (s n:ℕ),
+  ((List.map Prod.fst kvs) = List.range' s n  ) →
+(List.length kvs) = n :=
+by
+  induction kvs with
+  | nil =>
+    intro a b H
+    simp at H
+    symm at H
+    simp[List.range'_eq_nil] at H
+    aesop
+  | cons x xs Ih =>
+    intro s n H
+    simp at H
+    cases n with
+    | zero =>
+      have hh : List.range' s 0 = List.nil := by simp[List.range'_eq_nil]
+      rw[hh] at H
+      simp at H
+    | succ n' =>
+     rw[←List.range'_append] at H
+     simp at H
+     simp[Ih _ _ (And.right H)]
+
+
+lemma hrecord_elim : ∀ p kvs,
+  hrecord kvs p ==> hheader (List.length kvs) p ∗ hfields kvs p :=
+by
+  intro p kvs
+  unfold hrecord
+  xpull
+  intros z Hz
+  xsimp
+  apply himpl_of_eq
+  unfold maps_all_fields at Hz
+  simp[hrecord_elim_aux kvs 0 z Hz]
+
+
+
+def head : field := 0
+def tail : field := 1
+
+open trm prim
+
+
+def val_get_field  (k: field): val :=
+ [lang|
+ fun p =>
+    let p1 := p ++ 1 in
+    let q := p1 ++ ⟨Int.ofNat k⟩ in
+    !q]
+
+
+notation t1 "!." k:1525 => (val_get_field k) t1
+
+lemma triple_get_field : ∀ (p:loc) (k: field) v,
+  triple [lang| ⟨val_get_field k⟩ p]
+    (p. k ~~> v)
+    (fun r => ⌜r = v⌝  ∗ (p. k ~~> v))
+:=
+by
+    xwp
+    unfold hfield
+    xapp triple_ptr_add_nonneg
+    xwp
+    xapp triple_ptr_add_nonneg
+    sby xapp
+
+
+def val_set_field  (k: field): val :=
+ [lang|
+ fun p v =>
+    let p1 := p ++ 1 in
+    let q := p1 ++ ⟨Int.ofNat k⟩ in
+     q := v ]
+
+
+lemma triple_set_field : ∀ (p:loc) (k: field) v1 v2  ,
+  triple [lang| ⟨val_set_field k⟩ p v2]
+    (p. k ~~> v1)
+    (fun _ => (p. k ~~> v2))
+:=
+by
+    xwp
+    unfold hfield
+    xapp triple_ptr_add_nonneg
+    xwp
+    xapp triple_ptr_add_nonneg
+    sby xapp
+
+-- notation t1:5120 "." k:5120 " := " v:5120 => (val_set_field k) t1 v
+
+syntax:max lang noWs "." noWs ident : lang
+
+macro_rules
+  | `([lang| $rcrd.$f ])              =>
+    `(trm_val (val_get_field $f) [lang| $rcrd])
+  | `([lang| $rcrd.$f := $v ])        => `(trm_val (val_set_field $f) [lang| $rcrd] [lang| $v])
+
+example (t : val) (f : field) : trm := [lang| t.f]
+
+
+def hfields_lookup (k : field) (kvs : hrecord_fields) : Option val :=
+  match kvs with
+  | [] => none
+  | (ki, vi) :: kvs' => if k = ki then some vi else hfields_lookup k kvs'
+
+lemma triple_get_field_hfields : ∀ kvs (p:loc) k v,
+  hfields_lookup k kvs = some v →
+  triple [lang| ⟨val_get_field k⟩ p]
+    (hfields kvs p)
+    (fun r => ⌜r = v⌝  ∗  hfields kvs p) :=
+by
+intro L
+induction L with
+| nil => intro _ _ _ contra; simp[hfields_lookup] at contra
+| cons x L' ih =>
+  intro p f v E
+  simp[hfields_lookup] at E
+  cases Classical.em (f = x.1) with
+  | inl h =>
+    simp[(if_pos h)] at E
+    simp [←E]
+    simp[h]
+    apply triple_conseq_frame
+    { apply triple_get_field; aesop }
+    { simp[hfields]; xsimp }
+    { xsimp; simp[hfields, qstarE]; xsimp }
+  | inr h =>
+    apply triple_conseq_frame
+    simp[(if_neg h)] at E
+    { apply (ih _ _ _ E) }
+    { simp[hfields]; xsimp }
+    { simp[hfields, qstarE]
+      intro _; dsimp
+      xsimp }
+
+
+def hfields_update (k:field) (v:val) (kvs:hrecord_fields) : Option hrecord_fields :=
+  match kvs with
+  | List.nil => none
+  | kivi::kvs' => match kivi with
+                  | (ki, vi) => if k = ki
+                       then some ((k,v)::kvs')
+                       else match hfields_update k v kvs' with
+                            | none => none
+                            | some LR => some ((ki,vi)::LR)
+
+
+lemma triple_set_field_hfields : ∀ kvs kvs' k (p:loc) v,
+  hfields_update k v kvs = some kvs' →
+  triple [lang| ⟨val_set_field k⟩ p v]
+    (hfields kvs p)
+    (fun _ => hfields kvs' p) :=
+by
+  intro kvs
+  induction kvs with
+  | nil => intro _ _ _ _ contra; simp[hfields_update] at contra
+  | cons x kvs1 IH =>
+    intro kvs' k p v E
+    simp[hfields_update] at E
+    cases Classical.em (k = x.1) with
+    | inl h =>
+      simp[(if_pos h)] at E
+      simp [←E, h,hfields]
+      apply triple_frame
+      apply (triple_set_field p x.1 x.2 v)
+    | inr h =>
+      simp[(if_neg h)] at E
+      split at E
+      case h_1 a _ => simp at E
+      case h_2 kvs'' HH =>
+        simp at E
+        simp[←E]
+        apply triple_conseq_frame
+        { apply (IH _ _ _ _ HH) }
+        { simp[hfields]; xsimp }
+        { simp[hfields, qstarE]; intro _; xsimp; xsimp }
+
+
+
+
+lemma triple_get_field_hrecord : ∀ kvs (p:loc) k v,
+  hfields_lookup k kvs = some v →
+  triple [lang| (⟨val_get_field k⟩ p) ]
+    (hrecord kvs p)
+    (fun r => ⌜r = v⌝  ∗ hrecord kvs p) :=
+by
+  introv M
+  unfold hrecord
+  xtriple
+  xpull
+  intro z Hz
+  xapp (triple_get_field_hfields  _ _ _ _ M)
+  --xapp triple_get_field_hfields
+  /-
+  xapp_pre
+  eapply xapp_lemma; eapply (triple_get_field_hfields  _ _ _ _ M)
+  rotate_right; xapp_simp; hide_mvars=>//
+  -- xapp (triple_get_field_hfields  _ _ _ _ M)-/
+  xsimp
+  { simp }
+  { exact Hz }
+
+
+
+
+lemma hfields_update_preserves_fields : ∀ kvs kvs' k v,
+  hfields_update k v kvs = some kvs' →
+  List.map Prod.fst kvs' = List.map Prod.fst kvs :=
+by
+  intros kvs
+  induction kvs with
+  | nil => intro _ _ _ contra; simp[hfields_update] at contra
+  | cons kivi kvs1 ih =>
+    intro kvs' k v E
+    simp[hfields_update] at E
+    split at E
+    case cons.isTrue h => simp at E; simp[←E, h]
+    case cons.isFalse h =>
+      split at E
+      case h_1 a _ => simp at E
+      case h_2 kvs'' HH =>
+        simp at E
+        simp[←E]
+        simp[←(ih _ _ _  HH)]
+
+lemma hfields_update_preserves_maps_all_fields : ∀ kvs kvs' z k v,
+  hfields_update k v kvs = some kvs' →
+  maps_all_fields z kvs = maps_all_fields z kvs' :=
+by
+  intro kvs kvs' z k v M
+  unfold maps_all_fields
+  simp_all only [eq_iff_iff]
+  apply Iff.intro
+  case mp => intro a; simp[←a]; apply hfields_update_preserves_fields; apply M
+  case mpr => intro a; simp[←a]; symm; apply hfields_update_preserves_fields; apply M
+
+
+lemma triple_set_field_hrecord : ∀ kvs kvs' k (p:loc) v,
+  hfields_update k v kvs = some kvs' →
+  triple [lang| ⟨val_set_field k⟩ p v]
+    (hrecord kvs p)
+    (fun _ => hrecord kvs' p) :=
+by
+  introv M
+  unfold hrecord
+  xtriple
+  xpull
+  intros z Hz
+  xapp (triple_set_field_hfields  _ _ _ _ _ M)
+  xsimp
+  simp[←(hfields_update_preserves_maps_all_fields _ _ _ _ _ M)]
+  apply Hz
+
+
+
+
+lemma xapp_get_field_lemma : ∀ H k p Q,
+  (H ==> ∃ʰ kvs, (hrecord kvs p) ∗
+     (match hfields_lookup k kvs with
+     | none => ⌜False⌝
+     | some v => qwand (fun r => ⌜r = v ⌝  ∗ hrecord kvs p) (protect Q))) →
+     (H ==> wpgen_app [lang| ⟨val_get_field k⟩ p] Q):=
+by
+  intro H k p Q N
+  xchange N
+  intro kvs
+  generalize h :(hfields_lookup k kvs) = X
+  cases (X)
+  case none => xpull; intro contra; simp at contra
+  case some v =>
+    xsimp
+    apply triple_conseq_frame
+    { apply triple_get_field_hrecord; apply h }
+    { xsimp }
+    { apply qwand_cancel }
+
+
+
+lemma xapp_set_field_lemma : ∀ H k p v Q,
+  (H ==> ∃ʰ kvs, (hrecord kvs p) ∗
+     (match hfields_update k v kvs with
+     | none => ⌜False⌝
+     | some kvs' => qwand (fun _ => hrecord kvs' p) (protect Q))) →
+     (H ==> wpgen_app [lang| ⟨val_set_field k⟩ p v] Q):=
+by
+  intro H k p v Q N
+  xchange N
+  intro kvs
+  generalize h :(hfields_update k v kvs) = X
+  cases (X)
+  case none => xpull; intro contra; simp at contra
+  case some kvs' =>
+    xsimp
+    apply triple_conseq_frame
+    { apply triple_set_field_hrecord; apply h }
+    { xsimp }
+    { apply qwand_cancel }
+
+
+
+
+
+/-
+lemma eval_like_app_fix2 : ∀ (v0: val) v1 v2 f x1 x2 t1,
+  v0 = val_fix f x1 (trm_fun x2 t1) →
+  (x1 ≠ x2 ∧ f ≠ x2) →
+  eval_like (subst x2 v2 (subst x1 v1 (subst f v0 t1))) (trm_app (trm_app v0 v1) v2) :=
+by
+  intro v0 v1 v2 f x1 x2 t1 E N1N2
+  intro st Q h
+  refine eval.eval_app_arg1 st ([lang| v0 v1]) ([lang| v2]) ?Q1 Q ?_ ?_ ?_
+
+  apply eval_app_args
+  { apply eval_app_fix E; simp; simp[var_eq_spec];
+    apply eval_fun. }
+  { apply eval_val. }
+  { apply eval_app_fun. }
+-/
+
+  /-
+  xapp (triple_set_field_hfields)
+  xsimp
+  simp[←(hfields_update_preserves_maps_all_fields z M)]
+  -/
+/-
+def hfields_lookup (k : field) (kvs : hrecord_fields) : Option val :=
+  match kvs with
+  | [] => none
+  | (ki, vi) :: kvs' => if k = ki then some vi else hfields_lookup k kvs'
+
+lemma triple_get_field_hfields : ∀ kvs (p:loc) k v,
+  hfields_lookup k kvs = some v →
+  triple [lang| ⟨val_get_field k⟩ p]
+    (hfields kvs p)
+    (fun r => ⌜r = v⌝  ∗  hfields kvs p) :=
+by sorry
+-/
+/-
+lemma demo_hrecord_intro_elim : ∀ p x q,
+      (p ~~~> `{ head := x ; tail := q }) ==> ⌜True⌝ :=
+by
+ intro p x y
+ xchange hrecord_elim
+ sorry
+
+axiom triple_get_field_hrecord : ∀ (kvs : hrecord_fields) (p : loc) (k : field) (v : val),
+  hfields_lookup k kvs = some v →
+  triple (trm_app (val_get_field k) p) (hrecord kvs p) (fun r =>  ⌜r = v⌝ ∗ hrecord kvs p)
+
+-- Write Operation on Record fields
+axiom val_set_field : field→ val → val
+notation t1 ". " k " := " t2 => val_set_field k t1 t2
+
+def hfields_update (k : field) (v : val) (kvs : hrecord_fields) : Option hrecord_fields :=
+  match kvs with
+  | [] => none
+  | (ki, vi) :: kvs' =>
+    if k = ki then
+      some ((k, v) :: kvs')
+    else
+      match hfields_update k v kvs' with
+      | none => none
+      | some kvs'' => some ((ki, vi) :: kvs'')
+
+
+axiom triple_set_field_hrecord : ∀ (kvs kvs' : hrecord_fields) (k : field) (p : loc) (v : val),
+  hfields_update k v kvs = some kvs' →
+  triple (trm_app (val_set_field k p) v) (hrecord kvs p) (fun _ => hrecord kvs' p)
+
+-- Allocation of Records
+axiom val_alloc_hrecord : List field → trm
+
+axiom triple_alloc_hrecord : ∀ (ks : List field),
+  ks = List.range (List.length ks) →
+  triple (val_alloc_hrecord ks) emp (funloc p ↦ hrecord (List.map (fun k => (k,val_uninit)) ks) p)
+
+axiom val_new_hrecord_2 : field→ field→ val → val → val
+notation "`{" k1 " := " v1 "; " k2 " := " v2 "}" => val_new_hrecord_2 k1 k2 v1 v2
+
+axiom triple_new_hrecord_2 : ∀ (k1 k2 : field) (v1 v2 : val),
+  k1 = 0 →
+  k2 = 1 →
+  triple (`{ k1 := v1; k2 := v2 }) emp (funloc p ↦ p ~~~> `{ k1 := v1; k2 := v2 })
+
+axiom val_new_hrecord_3 : field→ field→ field→ val → val → val → val
+notation "`{" k1 " := " v1 "; " k2 " := " v2 "; " k3 " := " v3 "}" => val_new_hrecord_3 k1 k2 k3 v1 v2 v3
+
+axiom triple_new_hrecord_3 : ∀ (k1 k2 k3 : field) (v1 v2 v3 : val),
+  k1 = 0 →
+  k2 = 1 →
+  k3 = 2 →
+  triple (`{ k1 := v1; k2 := v2; k3 := v3 }) emp (funloc p ↦  p ~~~> `{ k1 := v1; k2 := v2; k3 := v3 })
+
+-- Deallocation of Records
+axiom val_dealloc_hrecord : val
+--notation "delete" => trm.val val_dealloc_hrecord
+
+axiom triple_dealloc_hrecord : ∀ (kvs : hrecord_fields) (p : loc),
+  triple (trm_app val_dealloc_hrecord p) (hrecord kvs p) (fun _ => emp)
+
+def jj (k : field) (kvs : hrecord_fields) (p:loc) (Q :  val → hProp): hProp :=
+match hfields_lookup k kvs with
+     | none =>  ⌜False⌝
+     | some v => (qwand (fun r => ⌜r = v⌝  ∗ hrecord kvs p) (protect Q))
+
+--axiom xapp_get_field_lemma : ∀ H k p Q,
+--  H ==> ∃ʰ kvs, (hrecord kvs p) ∗ (jj k kvs p Q) →
+--  H ==> wpgen_app (trm_app (val_get_field k) p) Q
+
+
+axiom xapp_set_field_lemma : ∀ H k p v Q,
+  (H ==> ∃ʰ kvs, (hrecord kvs p) ∗
+     match hfields_update k v kvs with
+     | none =>  ⌜False⌝
+     | some kvs' => qwand (fun _ => hrecord kvs' p) (protect Q) )→
+  H ==> wpgen_app (trm_app (val_set_field k p) v) Q
+-/
